%paper 2
\chapter{Hydrodynamic Relations}
\section{Normal Modes}
\label{App2}
\setcounter{equation}{0}

Here we derive the Eq. \eqref{normal-modes-eq} of the main text. In the parametrization \eqref{leading}, the left hand side of Eq.~\eqref{NS-eq} takes the form, 
\begin{align}\label{LHS}
\rho(\partial_t v+v\partial_zv) \approx \rho_0 \ddot{\phi}\, .
\end{align}
To linearize the right hand side of Eq.~\eqref{NS-eq} we note that the pressure is fixed by the density via the equation of state such that 
\begin{align}
P(z,t) = P[\rho(z,t)] \approx P[\rho_0(z)] - v_s^2[\rho_0(z)] (\rho_0 \phi)'\, ,
\end{align}
where the velocity $v_s$ is defined in Eq.~\eqref{v_s}.
At equilibrium, Eq.~\eqref{NS-eq} yields 
\begin{align}\label{cond}
v_s^2 \rho_0' = -\rho_0 U'
\end{align}
We have therefore,
\begin{align}
-P'-\rho U' \approx 
[ v_s^2 (\rho_0 \phi)']' +
(\rho_0 \phi)' U'
 \end{align}
Writing $(\rho_0 \phi)' U' =[ \rho_0 \phi U']' - \rho_0 \phi U''$ and using \eqref{cond} we obtain,
\begin{align}
-P'-\rho U' \approx 
[ v_s^2 \rho_0 \phi ']' 
- (\rho_0 \phi) U''
 \end{align}
Writing 
\begin{align*}
[ v_s^2 \rho_0 \phi ']'  =\rho_0 [ v_s^2 \phi ']' +  \rho_0' [ v_s^2 \phi ']
\end{align*}
and using \eqref{cond} again we obtain
\begin{align}\label{first}
-P'-\rho U' \approx 
\rho_0 [ v_s^2 \phi ']' -  
\rho_0 \phi ' U'
- \rho_0 \phi U''
 \end{align}
The third, viscosity term on the right hand side of Eq.~\eqref{NS-eq} reads
\begin{align}\label{third}
\partial_z(\eta\partial_z v) = [\eta \dot{\phi}']'
\end{align}
Substituting Eqs.~\eqref{LHS}, \eqref{first} and \eqref{third} in Eq.~\eqref{NS-eq} we obtain
\begin{align}
\ddot{\phi} = 
[ v_s^2 \phi ']' -  
 \phi ' U'
- \phi U'' + \rho_0^{-1} [\eta \dot{\phi}']'
\end{align}
For the solutions of the form $\phi(z,t) = e^{i \omega t} \chi'(z)$ we obtain the equation,
\begin{align}\label{interim}
 - \omega^2 \chi' = 
[ v_s^2 \chi'']' -  
\chi'' U'
- \chi' U'' +  (- i \omega)\rho_0^{-1} [\eta \chi'']'
\end{align}
Integration of Eq.~\eqref{interim} over $z$ yields Eq.~\eqref{normal-modes-eq}.

\section{Speed of Sound in a Free Degenerate 2D Ideal Fermi Gas}

At $T=0$ the free energy,
\be
F = E = V  \frac{  1}{ 4 \pi m}  \int_0^{p_F} d p p^3 = V  \frac{  1}{ 16 \pi m}  p_F^4
\ee
The density
\be\label{n}
n = \frac{p_F^2}{ 4 \pi}
\ee
so that 
\be
P = \frac{ \partial E }{ \partial V} = \pi n^2/m
\ee
\be
v_s^2 = 2 \pi n /  m^2 = \frac{p_F^2}{2  m^2 } = v_F^2/2 
\ee
In the parabolic confinement,
\be\label{hydro75}
v_s^2(z) = \frac{1}{2} v_F^2(z) = \frac{1 }{ m } E_F(z) = 
\frac{1}{m} (E_F - \frac{ k z^2 }{2} ) 
=
\frac{k}{ 2 m} (a^2 - z^2) = \frac{ \omega_{\perp}^2 }{2} (a^2 -z^2)
\ee

